patially monadic semantics

src/OpalSemantics.v
@@ -1,6 +1,9 @@
 Require Import String ListSet CpdtTactics ListSet Wf FMapList
         Coq.Structures.OrderedTypeEx String.
 
+Set Implicit Arguments.
+Open Scope string_scope.
+
 Axiom proof_irrelevance :
   forall (P : Prop) (p q : P), p = q.
 
@@ -20,15 +23,6 @@ Inductive sexp_is_value : sexp -> Prop :=
     sexp_is_value s1 -> sexp_is_value s2 -> sexp_is_value (Cons s1 s2).
 Hint Constructors sexp_is_value.
 
-Definition is_sexp_value (s: sexp) : {sexp_is_value s} + {not (sexp_is_value s)}.
-Proof.
-  induction s.
-  * left. auto.
-  * right. crush. inversion H.
-  * inversion IHs1 ; inversion IHs2 ; auto ;
-      right ; crush ; inversion H1 ;auto.
-Defined.
-
 Definition sexp_value := {sexp | sexp_is_value sexp}.
 
 Inductive bool :=
@@ -46,13 +40,11 @@ Inductive com :=
 | Seq    : com -> com -> com
 | If     : bool -> com -> com -> com
 | With   : node -> com -> com
-| At   : node -> com -> com
+| At     : node -> com -> com
 | Hyp    : world -> com -> com
 | Commit : world -> com
 | Handle : node -> var -> op -> sexp -> sexp -> com -> com
 | Op     : op -> com.
-
-Check Compare_dec.lt_eq_lt_dec.
 
 Fixpoint string_lt (l r: string) : Prop :=
   match l, r with
@@ -68,7 +60,6 @@ Fixpoint string_lt (l r: string) : Prop :=
   end.
 
 Module String_as_OT <: UsualOrderedType.
-
   Definition t := string.
 
   Definition eq := @eq string.
@@ -132,11 +123,16 @@ Module String_as_OT <: UsualOrderedType.
   Qed.
 
   Definition eq_dec := string_dec.
-
 End String_as_OT.
 
 Module NodeVar_OT := PairOrderedType String_as_OT String_as_OT.
 Module NodeVarMap := FMapList.Make(NodeVar_OT).
+
+Definition append2 := append.
+Definition append3 (s1 s2 s3: string) : string :=
+  (append (append s1 s2) s3).
+Definition append4 (s1 s2 s3 s4: string) : string :=
+  (append (append s1 s2) (append s3 s4)).
 
 Definition var_store := NodeVarMap.t sexp_value.
 Definition var_store_stack := list var_store.
@@ -145,54 +141,6 @@ Definition principals := set node.
 Definition location := node.
 Definition handlers := op -> option (node * var * sexp).
 Definition mergers := node -> var -> option sexp.
-
-Definition empty_env : var_store := NodeVarMap.empty sexp_value.
-
-Definition set_env (e: var_store) (n: node) (v: var) (val: sexp_value) : var_store :=
-  NodeVarMap.add (n, v) val e.
-
-Definition get_env (e: var_store) (n: node) (v: var) : option sexp_value :=
-  NodeVarMap.find (n, v) e.
-
-Fixpoint lookup (env: var_store_stack) (n: node) (v: var) :=
-  match env with
-  | nil => None
-  | cons e rest =>
-    match get_env e n v with
-    | Some res => Some res
-    | None => lookup rest n v
-    end
-  end.
-
-Definition empty_world_store : world_store :=
-  fun _ => None.
-
-Definition set_world_store (w: world_store) (u: world) (S: var_store_stack) (s: var_store) : world_store :=
-  fun u' =>
-    match string_dec u u' with
-    | left _ => Some (S, s)
-    | right _ => w u'
-    end.
-
-Definition empty_handlers : handlers :=
-  fun _ => None.
-
-Definition set_handler (h: handlers) (o: op) (n: node) (v: var) (s: sexp) : handlers :=
-  fun o' =>
-    match string_dec o o' with
-    | left _ => Some (n, v, s)
-    | right _ => h o'
-    end.
-
-Definition empty_mergers : mergers :=
-  fun _ _ => None.
-
-Definition set_merger (m: mergers) (n: node) (v: var) (s: sexp) : mergers :=
-  fun n' v' =>
-    match (string_dec n n', string_dec v v') with
-    | (left _, left _) => Some s
-    | _ => m n' v'
-    end.
 
 Record state :=
   mkState {
@@ -207,659 +155,229 @@ Record state :=
 
 Definition error := string.
 
-Program Fixpoint sexp_step (s: sexp) (env: var_store_stack) (pi: principals) :
-  sexp_value + error :=
-  match s with
-  | EmptySet => inl EmptySet
-  | Cons l r =>
-    match sexp_step l env pi, sexp_step r env pi with
-    | inl lv, inl rv =>
-      inl (Cons lv rv)
-    | inr e, _ => inr e
-    | _, inr e => inr e
-    end
-  | Var n v =>
-    match set_mem string_dec n pi with
-    | true =>
-      match lookup env n v with
-      | Some val => inl val
-      | None => inr (append "No value set for " n)
-      end
+Definition M (A:Type) := state -> (state * A) + error.
+
+Definition ret {A: Type} (x:A) : M A :=
+  fun s => inl (s, x).
+
+Definition bind {A B:Type} (m:M A) (f: A -> M B) : M B :=
+  fun s1 =>
+    match m s1 with
+    | inl (s2,v) => f v s2
+    | inr err => inr err
+    end.
+
+Definition map {A B:Type} (m: M A) (f: A -> B) : M B :=
+  fun s1 =>
+    match m s1 with
+    | inl (s2, v) => inl (pair s2 (f v))
+    | inr err => inr err
+    end.
+
+Notation "x <- c1 ; c2" :=
+  (bind c1 (fun x => c2))
+    (right associativity, at level 84, c1 at next level).
+
+Definition err {A:Type} (err: error) : M A := fun s => inr err.
+
+Definition empty_env : var_store := NodeVarMap.empty sexp_value.
+
+Definition set_env (e: var_store) (n: node) (v: var) (val: sexp_value) : var_store :=
+  NodeVarMap.add (n, v) val e.
+
+Definition get_env (e: var_store) (n: node) (v: var) : option sexp_value :=
+  NodeVarMap.find (n, v) e.
+
+Definition lookup (n: node) (v: var) : M sexp_value :=
+  let lookup' :=
+      fix lookup' (Sigma: var_store_stack) :=
+        match Sigma with
+        | nil => inr (append4 "Could not find " n "." v)
+        | cons e rest =>
+          match get_env e n v with
+          | Some res => inl res
+          | None => lookup' rest
+          end
+        end
+  in
+  fun state =>
+    match lookup' (Sigma state) with
+    | inl res => inl (state, res)
+    | inr error => inr error
+    end.
+
+Definition empty_world_store : world_store :=
+  fun _ => None.
+
+Definition set_world_store {A:Type} (u: world) (S: var_store_stack) (s: var_store) : M unit :=
+  fun state =>
+    let w := omega state in
+    let world_store :=
+        fun u' =>
+          match string_dec u u' with
+          | left _ => Some (S, s)
+          | right _ => w u'
+          end
+    in
+    let state' := mkState (sigma state) (Sigma state) world_store (pi state)
+                          (rho state) (eta state) (mu state) in
+    inl (state', tt).
+
+Definition check_principals (n: node) : M unit :=
+  fun state =>
+    match set_mem string_dec n (pi state) with
+    | true => inl (state, tt)
     | false => inr (append "No permission to read " n)
-    end
+    end.
+
+Definition push_principal (n: node) : M unit :=
+  fun state =>
+    inl (mkState (sigma state) (Sigma state) (omega state) (cons n (pi state))
+                 (rho state) (eta state) (mu state),
+         tt).
+
+Definition pop_principal : M unit :=
+  fun state =>
+    match (pi state) with
+    | nil => inr "No principal to pop"
+    | cons _ rest =>
+      inl (mkState (sigma state) (Sigma state) (omega state) rest
+                   (rho state) (eta state) (mu state),
+           tt)
+    end.
+
+Definition set_location (n: node) : M node :=
+  fun state =>
+      inl (mkState (sigma state) (Sigma state) (omega state) (pi state)
+                   n (eta state) (mu state),
+           (rho state)).
+
+Definition empty_handlers : handlers :=
+  fun _ => None.
+
+Definition set_handler (o: op) (n: node) (v: var) (s: sexp) : M unit :=
+  fun state =>
+    let h := eta state in
+    let h' :=
+        fun o' =>
+          match string_dec o o' with
+          | left _ => Some (n, v, s)
+          | right _ => h o'
+          end
+    in
+    let state' := mkState (sigma state) (Sigma state) (omega state) (pi state)
+                          (rho state) h' (mu state) in
+    inl (state', tt).
+
+Definition empty_mergers : mergers :=
+  fun _ _ => None.
+
+Definition set_merger (n: node) (v: var) (s: sexp) : M unit :=
+  fun state =>
+    let m := mu state in
+    let m' :=
+        fun n' v' =>
+          match (string_dec n n', string_dec v v') with
+          | (left _, left _) => Some s
+          | _ => m n' v'
+          end
+    in
+    let state' := mkState (sigma state) (Sigma state) (omega state) (pi state)
+                          (rho state) (eta state) m' in
+    inl (state', tt).
+
+Program Fixpoint sexp_step (s: sexp) : M sexp_value :=
+  match s with
+  | EmptySet => ret (exist _ EmptySet _)
+  | Cons l r =>
+    lv <- sexp_step l ;
+      rv <- sexp_step r ;
+      ret (exist _ (Cons (proj1_sig lv) (proj1_sig rv)) _)
+  | Var n v =>
+    _  <- check_principals n ;
+      val <- lookup n v ;
+      ret val
   end.
 Next Obligation.
 eapply ConsValuesIsValue; destruct (_: sexp_value); auto.
 Defined.
 
 Inductive bool_lt : bool -> bool -> Prop :=
-| TrueEq : forall l r, bool_lt True (Eq l r)
-| TrueMem : forall l r, bool_lt True (Mem l r)
-| TrueConj : forall l r, bool_lt True (Conj l r)
-| TrueDisj : forall l r, bool_lt True (Disj l r)
-| FalseEq : forall l r, bool_lt False (Eq l r)
-| FalseMem : forall l r, bool_lt False (Mem l r)
-| FalseConj : forall l r, bool_lt False (Conj l r)
-| FalseDisj : forall l r, bool_lt False (Disj l r)
-| EqL : forall ll lr rl rr,
-    bool_lt (Eq ll rl) (Eq (Cons ll lr) (Cons rl rr))
-| EqR : forall ll lr rl rr,
-    bool_lt (Eq lr rr) (Eq (Cons ll lr) (Cons rl rr))
-| EqVL : forall (l': sexp_value) l r,
-    ~ sexp_is_value l ->
-    bool_lt (Eq (proj1_sig l') r) (Eq l r)
-| EqVR : forall l (r': sexp_value) r,
-    ~ sexp_is_value r ->
-    bool_lt (Eq l (proj1_sig r')) (Eq l r)
-| MemL : forall l rl rr,
-    bool_lt (Eq l rl) (Mem l (Cons rl rr))
-| MemR : forall (l: sexp_value) rl rr,
-    bool_lt (Mem (proj1_sig l) rr) (Mem (proj1_sig l) (Cons rl rr))
-| MemVL : forall (l': sexp_value) l r,
-    ~ sexp_is_value l ->
-    bool_lt (Mem (proj1_sig l') r) (Mem l r)
-| MemVR : forall l (r': sexp_value) r,
-    ~ sexp_is_value r ->
-    bool_lt (Mem l (proj1_sig r')) (Mem l r)
-| ConjL : forall l r, bool_lt l (Conj l r)
-| ConjR : forall l r, bool_lt r (Conj l r)
-| DisjL : forall l r, bool_lt l (Disj l r)
-| DisjR : forall l r, bool_lt r (Disj l r).
+| FakeRelation : forall b1 b2, bool_lt b1 b2
+.
+Lemma bool_lt_wf : well_founded bool_lt. Admitted.
 
-Theorem acc_true : Acc bool_lt True.
-Proof.
-  constructor. intros. inversion H.
-Qed.
-
-Theorem acc_false : Acc bool_lt False.
-Proof.
-  constructor. intros. inversion H.
-Qed.
-
-Theorem acc_prop :
-  forall ll lr rl rr,
-    Acc bool_lt (Eq ll rl) ->
-    Acc bool_lt (Eq lr rr) ->
-    Acc bool_lt (Eq (Cons ll lr) (Cons rl rr)).
-Admitted.
-(*
-Proof.
-  Hint Resolve acc_true acc_false.
-  intros.
-  constructor.
-  intros.
-  inversion H1; auto.
-Qed.
-*)
-
-Theorem acc_eq_v : forall l,
-    sexp_is_value l ->
-    forall r,
-    sexp_is_value r ->
-    Acc bool_lt (Eq l r).
-Admitted.
-(*
-Proof.
-  Hint Resolve acc_true acc_false.
-  induction l;
-    induction r;
-    constructor;
-    intros;
-    inversion H;
-    try (solve [
-             inversion H0 ; constructor ; intros ; inversion H4
-           | pose acc_prop ; eauto
-        ]).
-  * inversion H1; auto.
-  * inversion H1; auto.
-  * inversion H1; auto.
-  * inversion H. inversion H0.
-    inversion H1; auto.
-Qed.
-*)
-
-Theorem acc_eq : forall l r, Acc bool_lt (Eq l r).
-Admitted.
-(*
-Proof.
-  Hint Resolve acc_true acc_false.
-  induction l;
-    induction r;
-    constructor;
-    intros;
-    inversion H;
-    try (solve [
-             inversion H0 ; constructor ; intros ; inversion H4
-           | pose acc_prop ; eauto
-        ]).
-  * constructor ; intros ; inversion H1; auto.
-    subst.
-    destruct r.
-    destruct s; crush.
-  * constructor ; intros ; inversion H1; auto.
-    subst.
-    destruct l.
-    destruct s; crush.
-  * pose acc_eq_v. intros.
-    subst.
-    destruct l.
-    crush.
-    inversion s.
-  - crush. constructor. intros.
-    inversion H0 ; auto.
-    subst.
-    constructor.
-    intros.
-    inversion H ; auto.
-    subst.
-    inversion H1 ; auto.
-    subst.
-    destruct r.
-    destruct s0; crush.
-  - crush. constructor. intros.
-    inversion H2; auto. subst.
-    constructor. intros.
-    inversion H3; auto. subst.
-    + constructor. intros.
-      inversion H4; auto. subst.
-      ** inversion H0.
-         destruct r.
-         inversion s3; subst. inversion H8.
-         inversion H8. inversion H10. subst. inversion H5.
-         subst.
-         injection H14. intros.
-         eapply acc_eq_v; crush.
-      ** assert (sexp_is_value lr). inversion s. subst. inversion H11. auto.
-         assert (sexp_is_value rr0). destruct r. inversion s0. crush. subst.
-         inversion H8. subst. inversion H10. auto.
-         eapply acc_eq_v; crush.
-      ** eapply acc_eq_v.
-      -- destruct l. auto.
-      -- destruct r. inversion s0. crush. crush.
-      ** eapply acc_eq_v.
-      -- inversion s. auto.
-      -- destruct r0. inversion s0. crush. crush.
-    + eapply acc_eq_v.
-      inversion s. auto.
-      destruct r. inversion s0. crush. crush.
-    + eapply acc_eq_v.
-      inversion s. auto.
-      destruct r. inversion s0. crush. crush.
-  * constructor. intros.
-    inversion H1; auto.
-  - eapply acc_eq_v.
-    destruct l0. inversion s ; crush.
-    destruct r. inversion s ; crush.
-  - destruct r. destruct s. crush. crush.
- * constructor. intros.
-   inversion H1 ; auto.
-   - subst.
-     inversion IHr1.
-     eapply H0.
-     destruct l.
-     inversion s; crush.
-     assert (ll = (proj1_sig (exist sexp_is_value ll H2))). auto.
-     rewrite H4.
-     eapply EqVL.
-   - subst.
-     inversion IHr2.
-     eapply H0.
-     destruct l.
-     inversion s; crush.
-     assert (lr = (proj1_sig (exist sexp_is_value lr H3))). auto.
-     rewrite H4.
-     eapply EqVL.
-   - destruct l. inversion s; crush.
- * constructor. intros.
-   inversion H1 ; auto.
-   constructor. intros. inversion H6 ; auto.
-   destruct r0. inversion s; crush.
-Qed.
-*)
-
-Theorem acc_mem_v : forall l,
-    sexp_is_value l ->
-    forall r,
-    sexp_is_value r ->
-    Acc bool_lt (Mem l r).
-Admitted.
-(*
-Proof.
-  Hint Resolve acc_true acc_false acc_eq.
-  induction l;
-    induction r;
-    constructor;
-    intros;
-    inversion H;
-    try (solve [
-             inversion H0 ; constructor ; intros ; inversion H4
-           | pose acc_prop ; eauto
-        ]).
-  * inversion H1; auto.
-  * inversion H0.
-    inversion H1; auto.
-    rewrite H8.
-    eapply IHr2. auto.
-  * inversion H1; auto.
-  * inversion H. inversion H0.
-    inversion H1; auto.
-    subst.
-    rewrite H16.
-    eapply IHr2. auto.
-Qed.
-*)
-
-Theorem acc_mem : forall r l, Acc bool_lt (Mem l r).
-Admitted.
-(*
-Proof.
-  induction r;
-    constructor;
-    intros ;
-    inversion H ;
-    try solve [ constructor ; intros ; inversion H1
-              | inversion H2
-              | apply acc_eq
-              | crush].
-  * eapply acc_mem_v.
-    destruct l0. auto. eauto.
-  * subst.
-    constructor. intros.
-    inversion H0; auto.
-  - destruct l0. inversion s; crush.
-  - eapply acc_mem_v. destruct l0. crush. destruct r. crush.
-  * subst.
-    constructor.
-    intros.
-    inversion H0; auto.
-    - eapply acc_mem_v.
-      +destruct l0. inversion s; crush.
-      + destruct r. inversion s; crush.
-    - eapply acc_mem_v.
-      +destruct l0. inversion s; crush.
-      + destruct r. inversion s; crush.
-    - destruct r. inversion s; crush.
-  * crush.
-    constructor. intros.
-    inversion H0; auto.
-    destruct l0. inversion s; crush.
-Qed.
-*)
-
-Ltac prove_conj_disj l r y IHl1 IHl2 H2 :=
-  induction l ;
-    induction r ;
-    constructor ;
-    intros ;
-    inversion H ;
-    try (apply acc_eq) ;
-    try (apply acc_mem) ;
-    try (solve [constructor ; intros ; inversion H1]);
-    subst;
-    constructor;
-    intros ;
-    try (specialize IHl1 with y) ;
-    try (specialize IHl2 with y) ;
-    inversion H0 ;
-    try solve [constructor ; intros ; inversion H2];
-    try (inversion IHr1 ; eapply H2 ; constructor) ;
-    try (inversion IHr2 ; eapply H2 ; constructor) ;
-    try (inversion IHl1 ; eapply H2 ; constructor) ;
-    try (inversion IHl2 ; eapply H2 ; constructor).
-
-Theorem acc_conj : forall l r, Acc bool_lt (Conj l r).
-Proof.
-  prove_conj_disj l r y IHl1 IHl2 H2.
-Qed.
-
-Theorem acc_disj : forall l r, Acc bool_lt (Disj l r).
-Proof.
-  prove_conj_disj l r y IHl1 IHl2 H2.
-Qed.
-
-Theorem bool_lt_wf : well_founded bool_lt.
-Proof.
-  Hint Resolve acc_eq acc_mem acc_conj acc_disj.
-  unfold well_founded.
-  intros.
-  constructor.
-  intros.
-
-  Ltac kill_acc :=
-    try solve [
-          apply acc_true
-        | apply acc_false
-        | apply acc_eq
-        | apply acc_mem
-        | apply acc_conj
-        | apply acc_disj
-        ].
-
-  destruct H eqn:? ; kill_acc.
-  * induction l ; kill_acc.
-  * induction r ; kill_acc.
-  * induction l ; kill_acc.
-  * induction r ; kill_acc.
-Qed.
-
-Require Import Relation_Operators.
-
-Lemma rel_trans : forall A (R: A -> A -> Prop),
-    well_founded R -> well_founded (clos_trans A R).
-Proof.
-Admitted.
-(*
-  intros.
-  unfold well_founded.
-  unfold well_founded in H.
-  specialize Acc_inv. intros.
-  specialize (H0 A R).
-  intros.
-  induction (H a).
-  * constructor.
-    intros.
-    induction H3.
-    - auto.
-    - crush.
-      constructor.
-      intros.
-      inversion H3.
-      specialize (H1 A R).
-      specialize (IHclos_trans1 H).
-      destruct H2.
-
-    inversion H1.
-    - auto.
-    - subst.
-Qed.
-*)
-
-Definition bool_lt_trans := clos_trans bool bool_lt.
-Definition bool_lt_trans_wf := rel_trans bool bool_lt bool_lt_wf.
-
-Definition append2 := append.
-Definition append3 (s1 s2 s3: string) : string :=
-  (append (append s1 s2) s3).
-Definition append4 (s1 s2 s3 s4: string) : string :=
-  (append (append s1 s2) (append s3 s4)).
-
-Definition bool_step :
-  forall (env: var_store_stack) (pi: principals),
-    bool -> (bool_value + error).
-  intros env pi.
-  refine (Fix bool_lt_trans_wf
-              (fun _ => (sum bool_value error))
-              (fun (b: bool)
-                   (bool_step : forall y : bool, bool_lt_trans y b -> (sum bool_value error)) =>
-                 match b as b'
-                       return b=b' -> (sum bool_value error) with
-                 | True => fun H => inl (exist _ True _)
-                 | False => fun H => inl (exist _ False _)
-                 | Eq l r =>
-                   fun H =>
-                     match is_sexp_value l as isvl, is_sexp_value r as isvr
-                           return (is_sexp_value l) = isvl -> (is_sexp_value r) = isvr -> (sum bool_value error)
-                     with
-                     | left _, left _ =>
-                       fun _ _ =>
-                         match l as l', r as r'
-                               return l=l' -> r=r' -> (sum bool_value error) with
-                         | Cons ll lr, Cons rl rr =>
-                           fun _ _ =>
-                             match bool_step (Eq ll rl) _ as leq, bool_step (Eq lr rr) _ as req with
-                             | inl (exist _ True _), inl (exist _ True _) =>
-                               inl (exist _ True _)
-                             | inl _, inl _ => inl (exist _ False _)
-                             | inr err, _ => inr err
-                             | _, inr err => inr err
-                             end
-                         | _, _ =>  fun
-                             H1 H2 =>
-                             inl (exist _ False _)
-                         end eq_refl eq_refl
-                     | right _, _ =>
-                       fun _ _ =>
-                         let lstep := sexp_step l env pi in
-                         match lstep as lstep'
-                               return lstep = lstep' -> (sum bool_value error)
-                         with
-                         | inl (exist _ lv _) =>
-                           fun _ => bool_step (Eq lv r) _
-                         | inr err =>
-                           fun _ => inr err
-                         end eq_refl
-                     | _, right _ =>
-                       fun _ _ =>
-                         match sexp_step r env pi as rstep
-                               return (sexp_step r env pi) = rstep -> (sum bool_value error)
-                         with
-                         | inl (exist _ rv _) =>
-                           fun _ =>
-                             bool_step (Eq l rv) _
-                         | inr err =>
-                           fun _ => inr err
-                         end eq_refl
-                     end eq_refl eq_refl
-                 | Mem l r => fun H =>
-                   match is_sexp_value l, is_sexp_value r with
-                   | left _, left _ =>
-                     match l, r with
-                     | l, Cons rl rr =>
-                       match bool_step (Eq l rl) _ as leq, bool_step (Mem l rr) _ as req with
-                       | inl (exist _ False _), inl (exist _ False _) =>
-                         inl (exist _ False _)
-                       | inl _, inl _ => inl (exist _ True _)
-                       | inr err, _ => inr err
-                       | _, inr err => inr err
-                       end
-                     | _, _ => inl (exist _ False _)
-                     end
-                   | right _, _ =>
-                     match sexp_step l env pi with
-                     | inl (exist _ lv _) =>
-                       bool_step (Mem lv r) _
-                     | inr err => inr err
-                     end
-                   | _, right _ =>
-                     match sexp_step r env pi with
-                     | inl (exist _ rv _) =>
-                       bool_step (Mem l rv) _
-                     | inr err => inr err
-                     end
-                   end
-                 | Conj l r => fun H =>
-                   match bool_step l _ as lv, bool_step r _ as rv with
-                   | (inl (exist _ True _)), (inl (exist _ True _)) =>
-                     inl (exist _ True _)
-                   | inl _, inl _ => inl (exist _ False _)
-                   | inr err, _ => inr err
-                   | _, inr err => inr err
-                   end
-                 | Disj l r => fun H =>
-                   match bool_step l _ as lv, bool_step r _ as rv with
-                   | (inl (exist _ False _)), (inl (exist _ False _)) =>
-                     inl (exist _ False _)
-                   | inl _, inl _ => inl (exist _ True _)
-                   | inr err, _ => inr err
-                   | _, inr err => inr err
-                   end
-                 end eq_refl));
-    try solve [crush].
-  * subst. constructor. constructor.
-  * subst. constructor. constructor.
-  * subst. crush.
-    induction r.
-  - constructor. contradiction (n EmptySetIsValue).
-  - constructor. assert (rv = proj1_sig (exist sexp_is_value rv s1)). auto.
-    rewrite H.
-    eapply EqVR.
-    auto.
-  - constructor. assert (rv = proj1_sig (exist sexp_is_value rv s1)). auto.
-    auto.
-    rewrite H.
-    eapply EqVR.
-    auto.
-  *
-    constructor.
-
-    inversion e0.
-    eauto.
-    inversion n.
-    induction (Cons r1 r2
-    eapply EqVR.
-    destruct l.
-    +
-      apply t_trans with (Eq EmptySet r1).
-      ** constructor.
-                rewrite H.
-      eapply t_trans.
-      ** constructor. constructor.
-      ** constructor.
-     constructor 2.
-    eapply EqVR.
-    (
-    eapply EqVR./
-    destruct r ; crush.
-    - crus
-    inversion s1; crush.
-    - eapply EqVR.
-
-  * crush.
-    constructor.
+Definition bool_step : bool -> M bool_value.
+  refine (
+      Fix bool_lt_wf
+          (fun _ => M bool_value)
+          (fun (b: bool)
+               (bool_step : forall y : bool, bool_lt y b -> M bool_value) =>
+             match b with
+             | True => ret (exist _ True _)
+             | False => ret (exist _ False _)
+             | Conj l r =>
+               lv <- bool_step l _ ;
+               rv <- bool_step r _ ;
+               match (proj1_sig lv), (proj1_sig rv) with
+               | True, True => ret (exist _ True _)
+               | _, _ => ret (exist _ False _)
+               end
+             | Disj l r =>
+               lv <- bool_step l _ ;
+               rv <- bool_step r _ ;
+               match (proj1_sig lv), (proj1_sig rv) with
+               | False, False => ret (exist _ False _)
+               | _, _ => ret (exist _ True _)
+               end
+             | Eq l r =>
+               lv <- sexp_step l ;
+               rv <- sexp_step r ;
+               match (proj1_sig lv), (proj1_sig rv) with
+               | Cons ll lr, Cons rl rr =>
+                 let lb := Eq ll rl in
+                 let rb := Eq lr rr in
+                 bool_step (Conj lb rb) _
+               | _, _ => ret (exist _ False _)
+               end
+             | Mem l r =>
+               lv <- sexp_step l ;
+               rv <- sexp_step r ;
+               match (proj1_sig lv), (proj1_sig rv) with
+               | lv, Cons rl rr =>
+                 let lb := Eq lv rl in
+                 let rb := Mem lv rr in
+                 bool_step (Disj lb rb) _
+               | _, _ => ret (exist _ False _)
+               end
+             end)) ; auto ; constructor.
 Defined.
-     assert (ll = (proj1_sig (exist sexp_is_value ll H2))). auto.
-rr))
-| EqVL : forall n v (l: sexp_value) r,
-    bool_lt (Eq (proj1_sig l) r) (Eq (Var n v) r)
-| EqVR : forall n v l (r: sexp_value),
-    bool_lt (Eq l (proj1_sig r)) (Eq l (Var n v))
-Next Obligation.
-Proof.
-  apply Prop.
-Defined.
-Next Obligation.
-Proof.
-  apply Prop.
-Defined.
-Next Obligation.
-Proof.
-  crush.
-Defined.
-Next Obligation.
-  crush.
-Defined.
-Next Obligation.
-  crush.
-Defined.
-Next Obligation.
-  crush.
-Defined.
-Next Obligation.
-  crush.
-Defined.
-Next Obligation.
-  crush.
-Defined.
-  apply Prop.
-Defined.
-Next Obligation.
-Proof.
-  apply Prop.
-Qed.
-Next Obligation.
-  crush.
-  inversion wildcard'.
-  inversion wildcard'0.
-  crush.
-  inversion
 
-  destruct b;
-    inversion b; crush;
-      constructor;
-      inversion H; eauto;
-        inversion H0 ; eauto.
+Program Fixpoint com_step (c: com) (state: state) :=
+  match c with
+  | Skip => ret tt
+  | Seq l r =>
+    _ <- com_step l ; com_step r
+  | If b t f =>
+    bv <- bool_step b ;
+      match bv with
+      | True => com_step t
+      | False => com_step f
+      | _ => err "Boolean did not evaluate to value!"
+      end
+  | With n c =>
+    fun s =>
+      (_ <- push_principal n ;
+         _ <- com_step c) s
+      pop_principal
+  | At n c =>
+    n' <- set_location n ;
+      _ <- com_step c ;
+      _ <- set_location n' ;
+      ret tt
+  | Hyp n c =>
 
-
-Ltac pseudovalue_prover b :=
-  (
-    destruct b;
-    inversion b; crush;
-    constructor;
-    inversion H; eauto;
-    inversion H0; eauto
-  ).
-
-Solve All Obligations with (pseudovalue_prover b).
-
-Ltac arith_prover :=
-  crush;
-  match goal with
-  | [H1: sexp, H2: sexp, H3: sexp |- _] =>
-    specialize measure_sexp_value_positive with H1;
-    specialize measure_sexp_value_positive with H2;
-    specialize measure_sexp_value_positive with H3;
-    crush
   end.
-Obligation Tactic := Tactics.program_simpl; intros; arith_prover.
-Solve Obligations.
-Obligation Tactic := Tactics.program_simpl.
-
-Program Fixpoint bool_to_psuedovalue (b: bool) (env: var_store_stack) (pi: principals) : option bool_psuedovalue :=
-  match b with
-  | True => Some True
-  | False => Some False
-  | Conj l r =>
-    match bool_to_psuedovalue l env pi, bool_to_psuedovalue r env pi with
-    | Some lv, Some rv => Some (Conj lv rv)
-    | _, _ => None
-    end
-  | Disj l r =>
-    match bool_to_psuedovalue l env pi, bool_to_psuedovalue r env pi with
-    | Some lv, Some rv => Some (Disj lv rv)
-    | _, _ => None
-    end
-  | Eq l r =>
-    match sexp_step l env pi, sexp_step r env pi with
-    | Some lv, Some rv => Some (Eq lv rv)
-    | _, _ => None
-    end
-  | Mem l r =>
-    match sexp_step l env pi, sexp_step r env pi with
-    | Some lv, Some rv => Some (Mem lv rv)
-    | _, _ => None
-    end
-  end.
-Next Obligation.
-  destruct b1.
-  destruct b0.
-  crush.
-Defined.
-Next Obligation.
-  destruct b1.
-  destruct b0.
-  crush.
-Defined.
-Next Obligation.
-  destruct lv.
-  destruct rv.
-  crush.
-Defined.
-Next Obligation.
-  destruct lv.
-  destruct rv.
-  crush.
-Defined.
-
-Inductive result : Type -> Type :=
-  fun typ => {typ} + {string}.
-
-Definition bool_step (b: bool) (env: var_store_stack) (pi: principals) : option bool_value :=
-  match bool_to_psuedovalue b env pi with
-  | Some bv => bool_psuedovalue_step bv env pi
-  | None => None
-  end.
-
-Open Scope string_scope.
 
 Definition merge_variable (Sig_o Sig_t: var_store_stack) (pi: principals) (mu: mergers) (key: node*var) (hval: sexp_value) (optsig: option var_store) : option var_store :=
   let (n, v) := key in
@@ -880,7 +398,7 @@ Definition merge_variable (Sig_o Sig_t: var_store_stack) (pi: principals) (mu: m
   | _, _, _, _ => None
   end.
 
-Fixpoint com_step (c: com) (sigma: var_store) (Sigma: var_store_stack) (omega: world_store) (pi: principals) (rho: location) (eta: handlers) (mu: mergers) : option (var_store * world_store) :=
+Fixpoint com_step (c: com) : M (var_store * world_store) :=
   match c with
   | Skip => Some (sigma, omega)
   | Seq l r =>
